% appendix.tex %
% Principal lemmas %

% ----------------------------------------------------------------------------

\section{Principal lemmas}
\label{PrincipalLemmas}

Binomial coefficients, \verb@CHOOSE@:
\begin{session}
\begin{verbatim}
CHOOSE_LESS = |- !n k. n < k ==> (CHOOSE n k = 0)

CHOOSE_SAME = |- !n. CHOOSE n n = 1
\end{verbatim}
\end{session}

Algebraic laws:
\begin{session}
\begin{verbatim}
RIGHT_CANCELLATION = 
|- !plus. Group plus ==> (!a b c. (plus b a = plus c a) ==> (b = c))

RING_0 = 
|- !plus times.
    RING(plus,times) ==>
    (!a. times(Id plus)a = Id plus) /\ (!a. times a(Id plus) = Id plus)
\end{verbatim}
\end{session}

\newpage
Scalar powers:
\begin{session}
\begin{verbatim}
POWER_1 = |- !plus. MONOID plus ==> (POWER plus 1 a = a)

POWER_DISTRIB = 
|- !plus times.
    RING(plus,times) ==>
    (!a b n. times a(POWER plus n b) = POWER plus n(times a b))

POWER_ADD = 
|- !plus.
    MONOID plus ==>
    (!m n a. POWER plus(m + n)a = plus(POWER plus m a)(POWER plus n a))
\end{verbatim}
\end{session}

Reduction of lists:
\begin{session}
\begin{verbatim}
REDUCE_APPEND = 
|- !plus.
    MONOID plus ==>
    (!as bs.
      REDUCE plus(APPEND as bs) = plus(REDUCE plus as)(REDUCE plus bs))

REDUCE_MAP_MULT = 
|- !plus times.
    RING(plus,times) ==>
    (!a bs. REDUCE plus(MAP(times a)bs) = times a(REDUCE plus bs))

REDUCE_MAP = 
|- !plus.
    MONOID plus /\ COMMUTATIVE plus ==>
    (!f g as.
      REDUCE plus(MAP(\k. plus(f k)(g k))as) =
      plus(REDUCE plus(MAP f as))(REDUCE plus(MAP g as)))
\end{verbatim}
\end{session}

Subranges of the natural numbers:
\begin{session}
\begin{verbatim}
RANGE_TOP = |- !n m. RANGE m(SUC n) = APPEND(RANGE m n)[m + n]

RANGE_SHIFT = |- !n m. RANGE(SUC m)n = MAP SUC(RANGE m n)
\end{verbatim}
\end{session}

\newpage
$\Sigma$-notation:
\begin{session}
\begin{verbatim}
SIGMA_ID = |- !plus m f. SIGMA(plus,m,0)f = Id plus

SIGMA_LEFT_SPLIT = 
|- !plus m n f. SIGMA(plus,m,SUC n)f = plus(f m)(SIGMA(plus,SUC m,n)f)

SIGMA_RIGHT_SPLIT = 
|- !plus.
    MONOID plus ==>
    (!m n f. SIGMA(plus,m,SUC n)f = plus(SIGMA(plus,m,n)f)(f(m + n)))

SIGMA_SHIFT = 
|- !plus m n f. SIGMA(plus,SUC m,n)f = SIGMA(plus,m,n)(f o SUC)

SIGMA_MULT_COMM = 
|- !plus times.
    RING(plus,times) ==>
    (!m n a f.
      times a(SIGMA(plus,m,n)f) = SIGMA(plus,m,n)((times a) o f))

SIGMA_PLUS_COMM = 
|- !plus.
    MONOID plus /\ COMMUTATIVE plus ==>
    (!f g m n.
      plus(SIGMA(plus,m,n)f)(SIGMA(plus,m,n)g) =
      SIGMA(plus,m,n)(\k. plus(f k)(g k)))

SIGMA_EXT = 
|- !plus.
    MONOID plus ==>
    (!f g m n.
      (!k. k < n ==> (f(m + k) = g(m + k))) ==>
      (SIGMA(plus,m,n)f = SIGMA(plus,m,n)g))
\end{verbatim}
\end{session}

Terms from the Binomial Theorem:
\begin{session}
\begin{verbatim}
BINTERM_0 = 
|- !plus times.
    RING(plus,times) ==>
    (!a b n. BINTERM plus times a b n 0 = POWER times n a)

BINTERM_n = 
|- !plus times.
    RING(plus,times) ==>
    (!a b n. BINTERM plus times a b n n = POWER times n b)
\end{verbatim}
\end{session}
